fix anchor element; add browser chrome
Signed-off-by: gterzian <2792687+gterzian@users.noreply.github.com>

content/src/boa/bindings/html_anchor_element.rs
@@ -1,0 +1,170 @@
+use boa_engine::{
+    Context, JsArgs, JsNativeError, JsResult, JsString, JsValue,
+    class::{Class, ClassBuilder},
+    js_string,
+    native_function::NativeFunction,
+    property::Attribute,
+};
+
+use crate::html::HTMLAnchorElement;
+
+use super::{
+    element::register_element_methods, event_target::register_event_target_methods,
+    html_element::register_html_element_methods,
+    hyperlink_element_utils::{document_creation_url, register_hyperlink_element_utils_methods},
+    node::register_node_methods,
+};
+
+impl Class for HTMLAnchorElement {
+    const NAME: &'static str = "HTMLAnchorElement";
+
+    fn data_constructor(
+        _this: &JsValue,
+        _args: &[JsValue],
+        _context: &mut Context,
+    ) -> JsResult<Self> {
+        Err(JsNativeError::typ()
+            .with_message("Illegal constructor")
+            .into())
+    }
+
+    fn init(class: &mut ClassBuilder<'_>) -> JsResult<()> {
+        register_event_target_methods(class)?;
+        register_node_methods(class)?;
+        register_element_methods(class)?;
+        register_html_element_methods(class)?;
+        register_hyperlink_element_utils_methods(class)?;
+        register_html_anchor_element_methods(class)
+    }
+}
+
+fn with_html_anchor_element_ref<R>(
+    this: &JsValue,
+    f: impl FnOnce(&HTMLAnchorElement) -> R,
+) -> JsResult<R> {
+    let object = this.as_object().ok_or_else(|| {
+        JsNativeError::typ().with_message("HTMLAnchorElement receiver is not an object")
+    })?;
+    let html_anchor_element = object
+        .downcast_ref::<HTMLAnchorElement>()
+        .ok_or_else(|| JsNativeError::typ().with_message("receiver is not an HTMLAnchorElement"))?;
+    Ok(f(&html_anchor_element))
+}
+
+fn register_html_anchor_element_methods(class: &mut ClassBuilder<'_>) -> JsResult<()> {
+    let realm = class.context().realm().clone();
+    class
+        .accessor(
+            js_string!("href"),
+            Some(NativeFunction::from_fn_ptr(get_href).to_js_function(&realm)),
+            Some(NativeFunction::from_fn_ptr(set_href).to_js_function(&realm)),
+            Attribute::all(),
+        )
+        .accessor(
+            js_string!("target"),
+            Some(NativeFunction::from_fn_ptr(get_target).to_js_function(&realm)),
+            Some(NativeFunction::from_fn_ptr(set_target).to_js_function(&realm)),
+            Attribute::all(),
+        )
+        .accessor(
+            js_string!("download"),
+            Some(NativeFunction::from_fn_ptr(get_download).to_js_function(&realm)),
+            Some(NativeFunction::from_fn_ptr(set_download).to_js_function(&realm)),
+            Attribute::all(),
+        )
+        .accessor(
+            js_string!("rel"),
+            Some(NativeFunction::from_fn_ptr(get_rel).to_js_function(&realm)),
+            Some(NativeFunction::from_fn_ptr(set_rel).to_js_function(&realm)),
+            Attribute::all(),
+        )
+        .accessor(
+            js_string!("referrerPolicy"),
+            Some(NativeFunction::from_fn_ptr(get_referrer_policy).to_js_function(&realm)),
+            Some(NativeFunction::from_fn_ptr(set_referrer_policy).to_js_function(&realm)),
+            Attribute::all(),
+        );
+    Ok(())
+}
+
+fn get_href(this: &JsValue, _: &[JsValue], context: &mut Context) -> JsResult<JsValue> {
+    let base_url = document_creation_url(context)?;
+    with_html_anchor_element_ref(this, |anchor| {
+        JsValue::from(JsString::from(anchor.href(&base_url)))
+    })
+}
+
+fn set_href(this: &JsValue, args: &[JsValue], context: &mut Context) -> JsResult<JsValue> {
+    let href = args
+        .get_or_undefined(0)
+        .to_string(context)?
+        .to_std_string_escaped();
+    with_html_anchor_element_ref(this, |anchor| anchor.set_href(&href))?;
+    Ok(JsValue::undefined())
+}
+
+fn get_target(this: &JsValue, _: &[JsValue], _: &mut Context) -> JsResult<JsValue> {
+    with_html_anchor_element_ref(this, |anchor| {
+        JsValue::from(JsString::from(anchor.target()))
+    })
+}
+
+fn set_target(this: &JsValue, args: &[JsValue], context: &mut Context) -> JsResult<JsValue> {
+    let target = args
+        .get_or_undefined(0)
+        .to_string(context)?
+        .to_std_string_escaped();
+    with_html_anchor_element_ref(this, |anchor| anchor.set_target(&target))?;
+    Ok(JsValue::undefined())
+}
+
+fn get_download(this: &JsValue, _: &[JsValue], _: &mut Context) -> JsResult<JsValue> {
+    with_html_anchor_element_ref(this, |anchor| {
+        JsValue::from(JsString::from(anchor.download()))
+    })
+}
+
+fn set_download(this: &JsValue, args: &[JsValue], context: &mut Context) -> JsResult<JsValue> {
+    let download = args
+        .get_or_undefined(0)
+        .to_string(context)?
+        .to_std_string_escaped();
+    with_html_anchor_element_ref(this, |anchor| anchor.set_download(&download))?;
+    Ok(JsValue::undefined())
+}
+
+fn get_rel(this: &JsValue, _: &[JsValue], _: &mut Context) -> JsResult<JsValue> {
+    with_html_anchor_element_ref(this, |anchor| {
+        JsValue::from(JsString::from(anchor.rel()))
+    })
+}
+
+fn set_rel(this: &JsValue, args: &[JsValue], context: &mut Context) -> JsResult<JsValue> {
+    let rel = args
+        .get_or_undefined(0)
+        .to_string(context)?
+        .to_std_string_escaped();
+    with_html_anchor_element_ref(this, |anchor| anchor.set_rel(&rel))?;
+    Ok(JsValue::undefined())
+}
+
+fn get_referrer_policy(this: &JsValue, _: &[JsValue], _: &mut Context) -> JsResult<JsValue> {
+    with_html_anchor_element_ref(this, |anchor| {
+        JsValue::from(JsString::from(anchor.referrer_policy()))
+    })
+}
+
+fn set_referrer_policy(
+    this: &JsValue,
+    args: &[JsValue],
+    context: &mut Context,
+) -> JsResult<JsValue> {
+    let referrer_policy = args
+        .get_or_undefined(0)
+        .to_string(context)?
+        .to_std_string_escaped();
+    with_html_anchor_element_ref(this, |anchor| {
+        anchor.set_referrer_policy(&referrer_policy)
+    })?;
+    Ok(JsValue::undefined())
+}
