content/src/boa/bindings/html_element.rs
@@ -1,0 +1,130 @@
+use boa_engine::{
+    Context, JsArgs, JsNativeError, JsResult, JsString, JsValue,
+    class::{Class, ClassBuilder},
+    js_string,
+    native_function::NativeFunction,
+    property::Attribute,
+};
+
+use crate::html::HTMLElement;
+
+use super::{
+    element::register_element_methods, event_target::register_event_target_methods,
+    node::register_node_methods,
+};
+
+impl Class for HTMLElement {
+    const NAME: &'static str = "HTMLElement";
+
+    fn data_constructor(
+        _this: &JsValue,
+        _args: &[JsValue],
+        _context: &mut Context,
+    ) -> JsResult<Self> {
+        Err(JsNativeError::typ()
+            .with_message("Illegal constructor")
+            .into())
+    }
+
+    fn init(class: &mut ClassBuilder<'_>) -> JsResult<()> {
+        register_event_target_methods(class)?;
+        register_node_methods(class)?;
+        register_element_methods(class)?;
+        register_html_element_methods(class)
+    }
+}
+
+fn with_html_element_ref<R>(this: &JsValue, f: impl FnOnce(&HTMLElement) -> R) -> JsResult<R> {
+    let object = this
+        .as_object()
+        .ok_or_else(|| JsNativeError::typ().with_message("HTMLElement receiver is not an object"))?;
+    let html_element = object
+        .downcast_ref::<HTMLElement>()
+        .ok_or_else(|| JsNativeError::typ().with_message("receiver is not an HTMLElement"))?;
+    Ok(f(&html_element))
+}
+
+pub(crate) fn register_html_element_methods(class: &mut ClassBuilder<'_>) -> JsResult<()> {
+    let realm = class.context().realm().clone();
+    class
+        .accessor(
+            js_string!("title"),
+            Some(NativeFunction::from_fn_ptr(get_title).to_js_function(&realm)),
+            Some(NativeFunction::from_fn_ptr(set_title).to_js_function(&realm)),
+            Attribute::all(),
+        )
+        .accessor(
+            js_string!("lang"),
+            Some(NativeFunction::from_fn_ptr(get_lang).to_js_function(&realm)),
+            Some(NativeFunction::from_fn_ptr(set_lang).to_js_function(&realm)),
+            Attribute::all(),
+        )
+        .accessor(
+            js_string!("dir"),
+            Some(NativeFunction::from_fn_ptr(get_dir).to_js_function(&realm)),
+            Some(NativeFunction::from_fn_ptr(set_dir).to_js_function(&realm)),
+            Attribute::all(),
+        )
+        .accessor(
+            js_string!("hidden"),
+            Some(NativeFunction::from_fn_ptr(get_hidden).to_js_function(&realm)),
+            Some(NativeFunction::from_fn_ptr(set_hidden).to_js_function(&realm)),
+            Attribute::all(),
+        );
+    Ok(())
+}
+
+fn get_title(this: &JsValue, _: &[JsValue], _: &mut Context) -> JsResult<JsValue> {
+    with_html_element_ref(this, |html_element| {
+        JsValue::from(JsString::from(html_element.title()))
+    })
+}
+
+fn set_title(this: &JsValue, args: &[JsValue], context: &mut Context) -> JsResult<JsValue> {
+    let title = args
+        .get_or_undefined(0)
+        .to_string(context)?
+        .to_std_string_escaped();
+    with_html_element_ref(this, |html_element| html_element.set_title(&title))?;
+    Ok(JsValue::undefined())
+}
+
+fn get_lang(this: &JsValue, _: &[JsValue], _: &mut Context) -> JsResult<JsValue> {
+    with_html_element_ref(this, |html_element| {
+        JsValue::from(JsString::from(html_element.lang()))
+    })
+}
+
+fn set_lang(this: &JsValue, args: &[JsValue], context: &mut Context) -> JsResult<JsValue> {
+    let lang = args
+        .get_or_undefined(0)
+        .to_string(context)?
+        .to_std_string_escaped();
+    with_html_element_ref(this, |html_element| html_element.set_lang(&lang))?;
+    Ok(JsValue::undefined())
+}
+
+fn get_dir(this: &JsValue, _: &[JsValue], _: &mut Context) -> JsResult<JsValue> {
+    with_html_element_ref(this, |html_element| {
+        JsValue::from(JsString::from(html_element.dir()))
+    })
+}
+
+fn set_dir(this: &JsValue, args: &[JsValue], context: &mut Context) -> JsResult<JsValue> {
+    let dir = args
+        .get_or_undefined(0)
+        .to_string(context)?
+        .to_std_string_escaped();
+    with_html_element_ref(this, |html_element| html_element.set_dir(&dir))?;
+    Ok(JsValue::undefined())
+}
+
+fn get_hidden(this: &JsValue, _: &[JsValue], _: &mut Context) -> JsResult<JsValue> {
+    with_html_element_ref(this, |html_element| JsValue::from(html_element.hidden()))
+}
+
+fn set_hidden(this: &JsValue, args: &[JsValue], _: &mut Context) -> JsResult<JsValue> {
+    let hidden = args.get_or_undefined(0).to_boolean();
+    with_html_element_ref(this, |html_element| html_element.set_hidden(hidden))?;
+    Ok(JsValue::undefined())
+}
