content/src/boa/bindings/hyperlink_element_utils.rs
@@ -1,0 +1,279 @@
+use boa_engine::{
+    Context, JsArgs, JsNativeError, JsResult, JsString, JsValue,
+    class::ClassBuilder,
+    js_string,
+    native_function::NativeFunction,
+    property::Attribute,
+};
+use url::Url;
+
+use crate::{dom::Document, html::{HTMLAnchorElement, HyperlinkElementUtils}};
+
+pub(crate) fn document_creation_url(context: &Context) -> JsResult<Url> {
+    let object = super::super::platform_objects::document_object(context)?;
+    let document = object
+        .downcast_ref::<Document>()
+        .ok_or_else(|| JsNativeError::typ().with_message("document object is not a Document"))?;
+    Ok(document.creation_url.clone())
+}
+
+fn with_hyperlink_element_utils_ref<R>(
+    this: &JsValue,
+    f: impl FnOnce(&dyn HyperlinkElementUtils) -> R,
+) -> JsResult<R> {
+    let object = this.as_object().ok_or_else(|| {
+        JsNativeError::typ().with_message("hyperlink receiver is not an object")
+    })?;
+    if let Some(anchor) = object.downcast_ref::<HTMLAnchorElement>() {
+        return Ok(f(&*anchor));
+    }
+    Err(JsNativeError::typ()
+        .with_message("receiver does not implement HyperlinkElementUtils")
+        .into())
+}
+
+pub(crate) fn register_hyperlink_element_utils_methods(
+    class: &mut ClassBuilder<'_>,
+) -> JsResult<()> {
+    let realm = class.context().realm().clone();
+    class
+        .accessor(
+            js_string!("origin"),
+            Some(NativeFunction::from_fn_ptr(get_origin).to_js_function(&realm)),
+            None,
+            Attribute::all(),
+        )
+        .accessor(
+            js_string!("protocol"),
+            Some(NativeFunction::from_fn_ptr(get_protocol).to_js_function(&realm)),
+            Some(NativeFunction::from_fn_ptr(set_protocol).to_js_function(&realm)),
+            Attribute::all(),
+        )
+        .accessor(
+            js_string!("username"),
+            Some(NativeFunction::from_fn_ptr(get_username).to_js_function(&realm)),
+            Some(NativeFunction::from_fn_ptr(set_username).to_js_function(&realm)),
+            Attribute::all(),
+        )
+        .accessor(
+            js_string!("password"),
+            Some(NativeFunction::from_fn_ptr(get_password).to_js_function(&realm)),
+            Some(NativeFunction::from_fn_ptr(set_password).to_js_function(&realm)),
+            Attribute::all(),
+        )
+        .accessor(
+            js_string!("host"),
+            Some(NativeFunction::from_fn_ptr(get_host).to_js_function(&realm)),
+            Some(NativeFunction::from_fn_ptr(set_host).to_js_function(&realm)),
+            Attribute::all(),
+        )
+        .accessor(
+            js_string!("hostname"),
+            Some(NativeFunction::from_fn_ptr(get_hostname).to_js_function(&realm)),
+            Some(NativeFunction::from_fn_ptr(set_hostname).to_js_function(&realm)),
+            Attribute::all(),
+        )
+        .accessor(
+            js_string!("port"),
+            Some(NativeFunction::from_fn_ptr(get_port).to_js_function(&realm)),
+            Some(NativeFunction::from_fn_ptr(set_port).to_js_function(&realm)),
+            Attribute::all(),
+        )
+        .accessor(
+            js_string!("pathname"),
+            Some(NativeFunction::from_fn_ptr(get_pathname).to_js_function(&realm)),
+            Some(NativeFunction::from_fn_ptr(set_pathname).to_js_function(&realm)),
+            Attribute::all(),
+        )
+        .accessor(
+            js_string!("search"),
+            Some(NativeFunction::from_fn_ptr(get_search).to_js_function(&realm)),
+            Some(NativeFunction::from_fn_ptr(set_search).to_js_function(&realm)),
+            Attribute::all(),
+        )
+        .accessor(
+            js_string!("hash"),
+            Some(NativeFunction::from_fn_ptr(get_hash).to_js_function(&realm)),
+            Some(NativeFunction::from_fn_ptr(set_hash).to_js_function(&realm)),
+            Attribute::all(),
+        );
+    Ok(())
+}
+
+fn get_origin(this: &JsValue, _: &[JsValue], context: &mut Context) -> JsResult<JsValue> {
+    let document_creation_url = document_creation_url(context)?;
+    with_hyperlink_element_utils_ref(this, |hyperlink| {
+        JsValue::from(JsString::from(hyperlink.origin(&document_creation_url)))
+    })
+}
+
+fn get_protocol(this: &JsValue, _: &[JsValue], context: &mut Context) -> JsResult<JsValue> {
+    let document_creation_url = document_creation_url(context)?;
+    with_hyperlink_element_utils_ref(this, |hyperlink| {
+        JsValue::from(JsString::from(hyperlink.protocol(&document_creation_url)))
+    })
+}
+
+fn set_protocol(this: &JsValue, args: &[JsValue], context: &mut Context) -> JsResult<JsValue> {
+    let document_creation_url = document_creation_url(context)?;
+    let value = args
+        .get_or_undefined(0)
+        .to_string(context)?
+        .to_std_string_escaped();
+    with_hyperlink_element_utils_ref(this, |hyperlink| {
+        hyperlink.set_protocol(&document_creation_url, &value)
+    })?;
+    Ok(JsValue::undefined())
+}
+
+fn get_username(this: &JsValue, _: &[JsValue], context: &mut Context) -> JsResult<JsValue> {
+    let document_creation_url = document_creation_url(context)?;
+    with_hyperlink_element_utils_ref(this, |hyperlink| {
+        JsValue::from(JsString::from(hyperlink.username(&document_creation_url)))
+    })
+}
+
+fn set_username(this: &JsValue, args: &[JsValue], context: &mut Context) -> JsResult<JsValue> {
+    let document_creation_url = document_creation_url(context)?;
+    let value = args
+        .get_or_undefined(0)
+        .to_string(context)?
+        .to_std_string_escaped();
+    with_hyperlink_element_utils_ref(this, |hyperlink| {
+        hyperlink.set_username(&document_creation_url, &value)
+    })?;
+    Ok(JsValue::undefined())
+}
+
+fn get_password(this: &JsValue, _: &[JsValue], context: &mut Context) -> JsResult<JsValue> {
+    let document_creation_url = document_creation_url(context)?;
+    with_hyperlink_element_utils_ref(this, |hyperlink| {
+        JsValue::from(JsString::from(hyperlink.password(&document_creation_url)))
+    })
+}
+
+fn set_password(this: &JsValue, args: &[JsValue], context: &mut Context) -> JsResult<JsValue> {
+    let document_creation_url = document_creation_url(context)?;
+    let value = args
+        .get_or_undefined(0)
+        .to_string(context)?
+        .to_std_string_escaped();
+    with_hyperlink_element_utils_ref(this, |hyperlink| {
+        hyperlink.set_password(&document_creation_url, &value)
+    })?;
+    Ok(JsValue::undefined())
+}
+
+fn get_host(this: &JsValue, _: &[JsValue], context: &mut Context) -> JsResult<JsValue> {
+    let document_creation_url = document_creation_url(context)?;
+    with_hyperlink_element_utils_ref(this, |hyperlink| {
+        JsValue::from(JsString::from(hyperlink.host(&document_creation_url)))
+    })
+}
+
+fn set_host(this: &JsValue, args: &[JsValue], context: &mut Context) -> JsResult<JsValue> {
+    let document_creation_url = document_creation_url(context)?;
+    let value = args
+        .get_or_undefined(0)
+        .to_string(context)?
+        .to_std_string_escaped();
+    with_hyperlink_element_utils_ref(this, |hyperlink| {
+        hyperlink.set_host(&document_creation_url, &value)
+    })?;
+    Ok(JsValue::undefined())
+}
+
+fn get_hostname(this: &JsValue, _: &[JsValue], context: &mut Context) -> JsResult<JsValue> {
+    let document_creation_url = document_creation_url(context)?;
+    with_hyperlink_element_utils_ref(this, |hyperlink| {
+        JsValue::from(JsString::from(hyperlink.hostname(&document_creation_url)))
+    })
+}
+
+fn set_hostname(this: &JsValue, args: &[JsValue], context: &mut Context) -> JsResult<JsValue> {
+    let document_creation_url = document_creation_url(context)?;
+    let value = args
+        .get_or_undefined(0)
+        .to_string(context)?
+        .to_std_string_escaped();
+    with_hyperlink_element_utils_ref(this, |hyperlink| {
+        hyperlink.set_hostname(&document_creation_url, &value)
+    })?;
+    Ok(JsValue::undefined())
+}
+
+fn get_port(this: &JsValue, _: &[JsValue], context: &mut Context) -> JsResult<JsValue> {
+    let document_creation_url = document_creation_url(context)?;
+    with_hyperlink_element_utils_ref(this, |hyperlink| {
+        JsValue::from(JsString::from(hyperlink.port(&document_creation_url)))
+    })
+}
+
+fn set_port(this: &JsValue, args: &[JsValue], context: &mut Context) -> JsResult<JsValue> {
+    let document_creation_url = document_creation_url(context)?;
+    let value = args
+        .get_or_undefined(0)
+        .to_string(context)?
+        .to_std_string_escaped();
+    with_hyperlink_element_utils_ref(this, |hyperlink| {
+        hyperlink.set_port(&document_creation_url, &value)
+    })?;
+    Ok(JsValue::undefined())
+}
+
+fn get_pathname(this: &JsValue, _: &[JsValue], context: &mut Context) -> JsResult<JsValue> {
+    let document_creation_url = document_creation_url(context)?;
+    with_hyperlink_element_utils_ref(this, |hyperlink| {
+        JsValue::from(JsString::from(hyperlink.pathname(&document_creation_url)))
+    })
+}
+
+fn set_pathname(this: &JsValue, args: &[JsValue], context: &mut Context) -> JsResult<JsValue> {
+    let document_creation_url = document_creation_url(context)?;
+    let value = args
+        .get_or_undefined(0)
+        .to_string(context)?
+        .to_std_string_escaped();
+    with_hyperlink_element_utils_ref(this, |hyperlink| {
+        hyperlink.set_pathname(&document_creation_url, &value)
+    })?;
+    Ok(JsValue::undefined())
+}
+
+fn get_search(this: &JsValue, _: &[JsValue], context: &mut Context) -> JsResult<JsValue> {
+    let document_creation_url = document_creation_url(context)?;
+    with_hyperlink_element_utils_ref(this, |hyperlink| {
+        JsValue::from(JsString::from(hyperlink.search(&document_creation_url)))
+    })
+}
+
+fn set_search(this: &JsValue, args: &[JsValue], context: &mut Context) -> JsResult<JsValue> {
+    let document_creation_url = document_creation_url(context)?;
+    let value = args
+        .get_or_undefined(0)
+        .to_string(context)?
+        .to_std_string_escaped();
+    with_hyperlink_element_utils_ref(this, |hyperlink| {
+        hyperlink.set_search(&document_creation_url, &value)
+    })?;
+    Ok(JsValue::undefined())
+}
+
+fn get_hash(this: &JsValue, _: &[JsValue], context: &mut Context) -> JsResult<JsValue> {
+    let document_creation_url = document_creation_url(context)?;
+    with_hyperlink_element_utils_ref(this, |hyperlink| {
+        JsValue::from(JsString::from(hyperlink.hash(&document_creation_url)))
+    })
+}
+
+fn set_hash(this: &JsValue, args: &[JsValue], context: &mut Context) -> JsResult<JsValue> {
+    let document_creation_url = document_creation_url(context)?;
+    let value = args
+        .get_or_undefined(0)
+        .to_string(context)?
+        .to_std_string_escaped();
+    with_hyperlink_element_utils_ref(this, |hyperlink| {
+        hyperlink.set_hash(&document_creation_url, &value)
+    })?;
+    Ok(JsValue::undefined())
+}
