content/src/html.rs
@@ -1,9 +1,11 @@
 mod environment_settings_object;
+mod hyperlink_element_utils;
 mod html_anchor_element;
 mod html_element;
 mod html_parser;
 
 pub use environment_settings_object::EnvironmentSettingsObject;
+pub(crate) use hyperlink_element_utils::HyperlinkElementUtils;
 pub use html_anchor_element::HTMLAnchorElement;
 pub use html_element::HTMLElement;
 pub use html_parser::{JsHtmlParserProvider, execute_parser_scripts, parse_html_into_document};
